improve performance by replacing dpair with refined pair for poset

iocy/event_structure.fst
@@ -11,7 +11,7 @@ type elem (a:Type) = id_typ * a
 unfold let el_id (x:elem 'a) : id_typ = fst x
 unfold let el_v (x:elem 'a) : 'a = snd x
 
-unfold let make_el (id:id_typ) (v:'a) = (id, v)
+unfold let make_el (id:id_typ) (v:'a) : elem 'a = (id, v)
 
 (** We need a set that allows the same value to appear multiple times and that allows
     us to distingusih between the appearances.
@@ -85,94 +85,81 @@ let _ = assert (__test_set1 `subset_set` __test_set2)
 let _ = assert (forall id v. make_el id v ∈ __test_set1 4 <==>
                       make_el id v ∈ __test_set2 8 /\ make_el (id+4) v ∈ __test_set2 8)
 
-type relation a = elem a -> elem a -> Type0
+type relation a (n:nat) = ofst:nat{ofst >= n} -> elem a -> elem a -> Type0
 
-(** non-strict partial order **)
-type partial_order (#a:Type) (#n:nat) (s:set a n) = ofst:nat{ofst >= n} -> rel:(relation a){
-  (forall x. x ∈ s ofst ==> x `rel` x) /\
-  (forall x y z. x ∈ s ofst /\ y ∈ s ofst /\ z ∈ s ofst ==> (x `rel` y /\ y `rel` z ==> x `rel` z)) /\
-  (forall x y. x ∈ s ofst /\ y ∈ s ofst ==> (x `rel` y /\ y `rel` x ==> x == y))
-}
-
-let empty_partial_order (#a:Type) (#n:nat) (s:set a n) : partial_order s =
+let empty_rel (#a:Type) (#n:nat) (s:set a n) : relation a n =
   fun ofst x y -> x ∈ s ofst /\ x == y
-
-let extend_partial_order
+  
+let extend_rel
   (#a:Type)
   (#n:nat)
-  (#s:set a n)
-  (po:partial_order s)
+  (s:set a n)
+  (po:relation a n)
   (ev1:(ofst:nat{ofst >= n} -> elem a){forall ofst. ev1 ofst ∈ s ofst})
   (ev2:(ofst:nat{ofst >= n} -> elem a){forall ofst. ev2 ofst ∈ s ofst})
-  : partial_order s =
+  : relation a n =
   fun ofst ev1' ev2' -> ev1' ∈ s ofst /\ ev2' ∈ s ofst /\ 
     (((ev2 ofst `po ofst` ev1 ofst ==> ev1 ofst == ev2 ofst) /\ (ev1' `po ofst` ev1 ofst /\ ev2 ofst `po ofst` ev2')) \/ (ev1' `po ofst` ev2'))
 
-type poset (a:Type) (n:nat) =
-  s:set a n
-  & po:partial_order s
-  & bot:option (ofst:nat{ofst >= n} -> elem a){(None? bot <==> n == 0)
-    /\ (Some? bot ==> (forall ofst. Some?.v bot ofst ∈ s ofst /\ (forall x. x ∈ s ofst ==> Some?.v bot ofst `po ofst` x)))}
-  & top_r:option (ofst:nat{ofst >= n} -> elem a){(None? top_r <==> n == 0) /\
-    (Some? top_r ==> (forall ofst. Some?.v top_r ofst ∈ s ofst /\ (forall x. x ∈ s ofst /\ x =!= Some?.v top_r ofst ==> ~(Some?.v top_r ofst `po ofst` x))))}
+type poset0 (a:Type) (n:nat) =
+  set a n
+  *
+  relation a n
+  *
+  option (ofst:nat{ofst >= n} -> elem a)
+  *
+  option (ofst:nat{ofst >= n} -> elem a)
 
-let empty_poset (#a:Type) : poset a 0 = (| empty_set, empty_partial_order empty_set, None, None |)
+type poset (a:Type) (n:nat) =
+  p:(poset0 a n){
+    let (s, rel, bot, top_r) = p in
+    (forall ofst x. x ∈ s ofst ==> x `rel ofst` x) /\
+    (forall ofst x y z. x ∈ s ofst /\ y ∈ s ofst /\ z ∈ s ofst ==> (x `rel ofst` y /\ y `rel ofst` z ==> x `rel ofst` z)) /\
+    (forall ofst x y. x ∈ s ofst /\ y ∈ s ofst ==> (x `rel ofst` y /\ y `rel ofst` x ==> x == y)) /\
+    (None? bot <==> n == 0) /\
+    (Some? bot ==> (forall ofst. Some?.v bot ofst ∈ s ofst /\ (forall x. x ∈ s ofst ==> Some?.v bot ofst `rel ofst` x))) /\
+    (None? top_r <==> n == 0) /\
+    (Some? top_r ==> (forall ofst. Some?.v top_r ofst ∈ s ofst /\ (forall x. x ∈ s ofst /\ x =!= Some?.v top_r ofst ==> ~(Some?.v top_r ofst `rel ofst` x))))
+  }
+
+let empty_poset (#a:Type) : poset a 0 = (empty_set, empty_rel empty_set, None, None)
 
 let return_poset (el:'e) : poset 'e 1 =
   let s = return_set el in
-  (| s, empty_partial_order s, Some (fun ofst -> make_el ofst el), Some (fun ofst -> make_el ofst el) |)
-
-
-let new_po0
-  (#n #m:nat)
-  (#s1:set 'e n)
-  (po1:partial_order s1)
-  (#s2:set 'e m)
-  (po2:partial_order s2)
-  (top_r1 : (ofst:nat{ofst >= n}) -> elem 'e)
-  (ofst:nat{ofst >= n + m})
-  : relation 'e = (fun x y ->
-  (x ∈ s1 (ofst-m) /\ y ∈ s1 (ofst-m) /\ x `po1 (ofst-m)` y) \/
-  (x ∈ s2 ofst /\ y ∈ s2 ofst /\ x `po2 ofst` y) \/
-  (x ∈ s1 (ofst-m) /\ y ∈ s2 ofst /\ x `po1 (ofst-m)` (top_r1 (ofst-m))))
+  (s, empty_rel s, Some (fun ofst -> make_el ofst el), Some (fun ofst -> make_el ofst el))
 
 let new_po
   (#n #m:nat)
-  (#s1:set 'e n)
-  (po1:partial_order s1)
-  (#s2:set 'e m)
-  (po2:partial_order s2)
-  (top_r1 : (ofst:nat{ofst >= n}) -> elem 'e) :
-  partial_order (s1 `union_set` s2) =
-  fun ofst -> 
-    let rel = new_po0 po1 po2 top_r1 ofst in
-    let s = s1 `union_set` s2 in
-    assert (forall x. x ∈ s ofst ==> x `rel` x);
-    assume (forall x y z. x ∈ s ofst /\ y ∈ s ofst /\ z ∈ s ofst ==> (x `rel` y /\ y `rel` z ==> x `rel` z));
-    assert (forall x y. x ∈ s ofst /\ y ∈ s ofst ==> (x `rel` y /\ y `rel` x ==> x == y));
-    rel
-
+  (s1:set 'e n)
+  (rel1:relation 'e n)
+  (s2:set 'e m)
+  (rel2:relation 'e m)
+  (top_r1 : (ofst:nat{ofst >= n}) -> elem 'e)
+  : relation 'e (n+m) = (fun (ofst:nat{ofst >= n + m}) x y ->
+  (x ∈ s1 (ofst-m) /\ y ∈ s1 (ofst-m) /\ x `rel1 (ofst-m)` y) \/
+  (x ∈ s2 ofst /\ y ∈ s2 ofst /\ x `rel2 ofst` y) \/
+  (x ∈ s1 (ofst-m) /\ y ∈ s2 ofst /\ x `rel1 (ofst-m)` (top_r1 (ofst-m))))
 
 let append_poset (#n #m:nat) (pos1:poset 'e n) (pos2:poset 'e m) : poset 'e (n+m) =
-  let (| s1, po1, bot1, top_r1 |) = pos1 in
-  let (| s2, po2, bot2, top_r2 |) = pos2 in
+  let (s1, rel1, bot1, top_r1)  = pos1 in
+  let (s2, rel2, bot2, top_r2) = pos2 in
   match bot1, bot2 with
   | None, None
   | None, _ -> pos2
   | _, None -> pos1
   | _, _ -> begin
     let s = s1 `union_set` s2 in
-    let po : partial_order s = new_po po1 po2 (Some?.v top_r1) in
+    let rel : relation 'e (n+m) = new_po s1 rel1 s2 rel2 (Some?.v top_r1) in
     let bot = Some (fun (ofst:nat{ofst >= n+m}) -> Some?.v bot1 (ofst-m)) in
     let top = Some (fun (ofst:nat{ofst >= n+m}) -> Some?.v top_r2 ofst) in
-    (| s1 `union_set` s2, po, bot , top |)
+    (s1 `union_set` s2, rel, bot , top)
   end
 
 let subset_poset (#n #m:nat) (pos1:poset 'e n) (pos2:poset 'e m) : Type0 =
-  let (| s1, po1, bot1, top_r1 |) = pos1 in
-  let (| s2, po2, bot2, top_r2 |) = pos2 in
+  let (s1, rel1, bot1, top_r1) = pos1 in
+  let (s2, rel2, bot2, top_r2) = pos2 in
   s1 `subset_set` s2 /\
-  (forall ofst x y. x ∈ s1 ofst /\ y ∈ s1 ofst /\ x `po1 ofst` y ==> x `po2 ofst` y)
+  (forall ofst x y. x ∈ s1 ofst /\ y ∈ s1 ofst /\ x `rel1 ofst` y ==> x `rel2 ofst` y)
   
 type trace 'e = list 'e
   
@@ -181,18 +168,18 @@ type marked = id_typ -> Type0
 let empty_marked : marked = fun _ -> False
 
 let mark (m:marked) (v:id_typ) : marked = fun v' -> v == v' \/ m v'
-
+  
 let rec test_membership0 (t:trace int) (#n:nat) (p:poset int n) (el_prev:elem int) (marked_ids:marked) : Type0 =
-  let (| s, po, bot, top |) = p in
+  let (s, rel, _, _) = p in
   match t with
   | [] -> True
   | h :: tl -> exists id_h. ~(marked_ids id_h) /\ 
                       (make_el id_h h ∈ s n) /\
-                      ((el_prev `po n` make_el id_h h) \/ ~(make_el id_h h `po n` el_prev)) /\
+                      ((el_prev `rel n` make_el id_h h) \/ ~(make_el id_h h `rel n` el_prev)) /\
                       test_membership0 tl p (make_el id_h h) (mark marked_ids id_h)
 
 let test_membership (t:trace int) (#n:nat) (p:poset int n) : Type0 =
-  let (| s, po, bot, top |) = p in
+  let (s, _, bot, _) = p in
   match t with
   | [] -> n == 0
   | h :: tl -> Some? bot /\ (let b = Some?.v bot n in
@@ -202,13 +189,13 @@ let test_membership (t:trace int) (#n:nat) (p:poset int n) : Type0 =
     | \
     2  3 **)
 let __test_set : set int 3 = ((empty_set ⊕ 1) ⊕ 2) ⊕ 3
-let __test_po : partial_order __test_set =
-  extend_partial_order
-    (extend_partial_order (empty_partial_order __test_set) (fun id -> make_el (id-2) 1) (fun id -> make_el (id-1) 2))
+let __test_po : relation int 3 =
+  extend_rel __test_set
+    (extend_rel __test_set (empty_rel __test_set) (fun id -> make_el (id-2) 1) (fun id -> make_el (id-1) 2))
     (fun id -> make_el (id-2) 1) (fun id -> make_el id 3)
 
 let __test_poset : poset int 3 =
-  (| __test_set, __test_po, Some (fun (ofst:nat{ofst >= 3}) -> make_el (ofst-2) 1), Some (fun id -> make_el id 3) |)
+  (__test_set, __test_po, Some (fun (ofst:nat{ofst >= 3}) -> make_el (ofst-2) 1), Some (fun id -> make_el id 3))
 
 let _ =
   assert ([1;2] `test_membership` __test_poset);
@@ -231,18 +218,17 @@ let _ = assert (~([3;1;2] `test_membership` __test_poset))
        4 **)
        
 let __test_set3 : set int 4 = (((return_set 1) ⊕ 2) ⊕ 3) ⊕ 4
-let __test_po3 : partial_order __test_set3 =
-  extend_partial_order 
-    (extend_partial_order
-        (extend_partial_order
-        (extend_partial_order (empty_partial_order __test_set3) (fun id -> make_el (id-3) 1) (fun id -> make_el (id-2) 2))
+let __test_po3 : relation int 4 =
+  extend_rel __test_set3
+    (extend_rel __test_set3
+        (extend_rel __test_set3
+        (extend_rel __test_set3 (empty_rel __test_set3) (fun id -> make_el (id-3) 1) (fun id -> make_el (id-2) 2))
         (fun id -> make_el (id-3) 1) (fun id -> make_el (id-1) 3))
       (fun id -> make_el (id-1) 3) (fun id -> make_el id 4))
     (fun id -> make_el (id-2) 2) (fun id -> make_el id 4)
 
-#set-options "--z3rlimit 12"
 let __test_poset3 : poset int 4 =
-  (| __test_set3, __test_po3, Some (fun (ofst:nat{ofst >= 4}) -> make_el (ofst-3) 1), Some (fun id -> make_el id 4) |)
+  (__test_set3, __test_po3, Some (fun (ofst:nat{ofst >= 4}) -> make_el (ofst-3) 1), Some (fun id -> make_el id 4)) 
 
 let _ =
   assert ([1;2;3;4] `test_membership` __test_poset3)
@@ -265,7 +251,7 @@ type event_typ 'e = option (nat * 'e)
 
 let op (e:'e) (th_id:nat) : poset (event_typ 'e) 1 =
   let s = return_set (Some (th_id, e)) in
-  (| s, empty_partial_order s, Some (fun ofst -> make_el ofst (Some (th_id, e))), Some (fun ofst -> make_el ofst (Some (th_id, e))) |)
+  (s, empty_rel s, Some (fun ofst -> make_el ofst (Some (th_id, e))), Some (fun ofst -> make_el ofst (Some (th_id, e))))
 
 
 (**
@@ -273,7 +259,7 @@ let op (e:'e) (th_id:nat) : poset (event_typ 'e) 1 =
       |             async                   /        \
       |          ---------->               /          \
       |                                   v           v
-      v                              bot (ofst-2)   make_el ofst None    (new top)
+      v                              bot (ofst-2)   make_el ofst None    (new top_r)
      top_r ofst                            |
                                           |
                                           v
@@ -281,33 +267,33 @@ let op (e:'e) (th_id:nat) : poset (event_typ 'e) 1 =
 **)
 
 let async (#n:nat) (p:poset (event_typ 'e) n) : poset (event_typ 'e) (n+2) = 
-  let (| s, po, bot, top_r |) = p in
+  let (s, rel, bot, top_r) = p in
   let s' = (s ⊕ None) ⊕ None in
   assert (forall ofst. make_el ofst None ∈ s' ofst /\ make_el (ofst-1) None ∈ s' ofst);
-  let po : partial_order s' = (fun ofst x y -> (x == make_el (ofst-1) None /\ y ∈ s' ofst) \/
+  let rel' : relation (event_typ 'e) (n+2) = (fun ofst x y -> (x == make_el (ofst-1) None /\ y ∈ s' ofst) \/
                                             (x == make_el ofst None /\ y == make_el ofst None) \/
-                                            (x ∈ s (ofst-2) /\ y ∈ s (ofst-2) /\ x `po (ofst-2)` y)) in
-  (| s', po, Some (fun (ofst:nat{ofst >= n+2}) -> make_el (ofst-1) None), Some (fun ofst -> make_el ofst None) |)
+                                            (x ∈ s (ofst-2) /\ y ∈ s (ofst-2) /\ x `rel (ofst-2)` y)) in
+  (s', rel', Some (fun (ofst:nat{ofst >= n+2}) -> make_el (ofst-1) None), Some (fun ofst -> make_el ofst None))
 
 (** CA: Not very principled since the po is defined over xs and ys which are not part of S **)
 let await (#e:Type) (th_id:nat) : poset (event_typ e) 1 =
   let s : set (event_typ e) 1 = return_set None in
-  let po : partial_order s = (fun ofst x y -> (x ∈ s ofst /\ y ∈ s ofst) \/ (y == make_el ofst None /\ Some? (el_v x) /\ fst (Some?.v (el_v x)) == th_id)) in
-  (| s, po, Some (fun ofst -> make_el ofst None), Some (fun ofst -> make_el ofst None) |)
+  let rel = (fun ofst x y -> (x ∈ s ofst /\ y ∈ s ofst) \/ (y == make_el ofst None /\ Some? (el_v x) /\ fst (Some?.v (el_v x)) == th_id)) in
+  (s, rel, Some (fun ofst -> make_el ofst None), Some (fun ofst -> make_el ofst None))
 
 let rec membership0 (t:trace 'e) (#n:nat) (p:poset (event_typ 'e) n) (el_prev:elem (event_typ 'e)) (marked_ids:marked) : Type0 =
-  let (| s, po, bot, top |) = p in
+  let (s, rel, _, _) = p in
   match t with
   | [] -> True
   | ev :: tl -> exists id_ev id_th. 
                       ~(marked_ids id_ev) /\ 
                       (let el = make_el id_ev (Some (id_th, ev)) in
                         (el ∈ s n) /\
-                        ((el_prev `po n` el) \/ ~(el `po n` el_prev)) /\
+                        ((el_prev `rel n` el) \/ ~(el `rel n` el_prev)) /\
                         membership0 tl p el (mark marked_ids id_ev))
 
 let membership (t:trace 'e) (#n:nat) (p:poset (event_typ 'e) n) : Type0 =
-  let (| s, po, bot, top |) = p in
+  let (s, _, bot, _) = p in
   match t with
   | [] -> n == 0
   | h :: tl -> Some? bot /\ (let bot_el = Some?.v bot n in
@@ -315,11 +301,9 @@ let membership (t:trace 'e) (#n:nat) (p:poset (event_typ 'e) n) : Type0 =
               | None -> membership0 t p bot_el (mark empty_marked (el_id bot_el))
               | Some b' -> h == snd b' /\ membership0 tl p bot_el (mark empty_marked (el_id bot_el)))
 
-#reset-options
-
 let prog0 () : poset (event_typ int) 3 = async (op 2 2)
 let __test_prog0 () = 
-  let (| s, po, bot, top_r |) = prog0 () in
+  let (s, _, bot, top_r) = prog0 () in
   assert (Some? bot /\ Some?.v bot 3 == make_el 2 None);
   assert (Some? top_r /\ Some?.v top_r 3 == make_el 3 None);
   assert (make_el 1 (Some (2,2)) ∈ s 3);
@@ -329,7 +313,7 @@ let __test_prog0 () =
 let prog01 () : poset (event_typ int) 4 = op 1 1 `append_poset` async (op 2 2)
 
 let __test_prog01 () = 
-  let (| s, po, bot, top_r |) = prog01 () in
+  let (s, _, bot, top_r) = prog01 () in
   assert (Some? bot /\ Some?.v bot 4 == make_el 1 (Some (1,1)));
   assert (Some? top_r /\ Some?.v top_r 4 == make_el 4 None);
   assert (make_el 1 (Some (1,1)) ∈ s 4);
@@ -340,7 +324,7 @@ let __test_prog01 () =
 let prog02 () : poset (event_typ int) 4 = async (op 2 2) `append_poset` op 1 1
 
 let __test_prog02 () = 
-  let (| s, po, bot, top_r |) = prog02 () in
+  let (s, _, bot, top_r) = prog02 () in
   assert (Some? bot /\ Some?.v bot 4 == make_el 2 None);
   assert (Some? top_r /\ Some?.v top_r 4 == make_el 4 (Some (1,1)));
   assert (make_el 1 (Some (2,2)) ∈ s 4);
@@ -351,7 +335,7 @@ let __test_prog02 () =
 let prog03 () : poset (event_typ int) 5 = (async (op 2 2) `append_poset` op 1 1) `append_poset` op 3 1
 
 let __test_prog03 () = 
-  let (| s, po, bot, top_r |) = prog03 () in
+  let (s, _, bot, top_r) = prog03 () in
   assert (Some? bot /\ Some?.v bot 5 == make_el 2 None);
   assert (Some? top_r /\ Some?.v top_r 5 == make_el 5 (Some (1,3)));
   assert (make_el 1 (Some (2,2)) ∈ s 5);
@@ -362,8 +346,9 @@ let __test_prog03 () =
 
 let prog04 () : poset (event_typ int) 5 = (op 1 1 `append_poset` async (op 2 2)) `append_poset` op 3 1
 
+#set-options "--z3rlimit 64"
 let __test_prog04 () = 
-  let (| s, po, bot, top_r |) = prog04 () in
+  let (s, _, bot, top_r) = prog04 () in
   assert (Some? bot /\ Some?.v bot 5 == make_el 1 (Some (1,1)));
   assert (Some? top_r /\ Some?.v top_r 5 == make_el 5 (Some (1,3)));
   assert (make_el 1 (Some (1,1)) ∈ s 5);
@@ -375,7 +360,7 @@ let __test_prog04 () =
 let prog05 () : poset (event_typ int) 4 = async (op 2 2) `append_poset` await 2
 
 let __test_prog05 () = 
-  let (| s, po, bot, top_r |) = prog05 () in
+  let (s, _, bot, top_r) = prog05 () in
   assert (Some? bot /\ Some?.v bot 4 == make_el 2 None);
   assert (Some? top_r /\ Some?.v top_r 4 == make_el 4 None);
   assert (make_el 1 (Some (2,2)) ∈ s 4);
@@ -399,36 +384,31 @@ let __test_prog05 () =
 
 let prog1 () : poset (event_typ int) 7 = (((op 1 1 `append_poset` async (op 2 2)) `append_poset` (op 3 1)) `append_poset` await 2) `append_poset` op 4 1
 
-let __test_prog1 () = 
-  let (| s, po, bot, top_r |) = prog1 () in
-  assert (Some? bot /\ Some?.v bot 7 == make_el 1 (Some (1,1)));
-  assert (Some? top_r /\ Some?.v top_r 7 == make_el 7 (Some (1,4)));
-  assert (make_el 1 (Some (1,1)) ∈ s 7);
-  assert (make_el 5 (Some (1,3)) ∈ s 7);
-  assert (make_el 6 None ∈ s 7);
-  assert (make_el 7 (Some (1,4)) ∈ s 7)
-
 // TODO: why do I have performance problems here?
 // TODO: test on a smaller case if await works:
 //        (async (op 2 2)) `append_poset` await 2) `append_poset` op 4 1
 //           assert ([2;4] `membership` _)
 //           assert (~([4;2] `membership` _)
-#set-options "--z3rlimit 64"
-let __test_prog1'' () = 
-  let (| s, po, bot, top_r |) = (((op 1 1 `append_poset` async (op 2 2)) `append_poset` (op 3 1)) `append_poset` await 2) `append_poset` op 4 1 in
+let __test_prog1 () = 
+  let (s, po, bot, top_r) = prog1 () in
   assert (Some? bot /\ Some?.v bot 7 == make_el 1 (Some (1,1)));
   assert (Some? top_r /\ Some?.v top_r 7 == make_el 7 (Some (1,4)));
+  assert (make_el 1 (Some (1,1)) ∈ s 7);
+  assert (make_el 5 (Some (1,3)) ∈ s 7);
+  assert (make_el 6 None ∈ s 7);
+  assert (make_el 7 (Some (1,4)) ∈ s 7);
   assert (make_el 2 (Some (2,2)) ∈ s 7);
   assert (make_el 3 None ∈ s 7);
   assert (make_el 4 None ∈ s 7)
+
 
 let _ = assert ([1;4] `membership` prog1 ()) 
   
 let _ = assert (~([4;1] `membership` prog1 ()))
 
-#set-options "--z3rlimit 64"
+//#set-options "--z3rlimit 512 --fuel 200 --ifuel 200"
 let _ = assert ([1;2;3;4] `membership` prog1 ())
 
 let _ = assert ([1;3;2;4] `membership` prog1 ())
 
-let _ = assert ([1;3;4;2] `membership` prog1 ()) 
+let _ = assert (~([1;3;4;2] `membership` prog1 ())) 
